thys/Clean/examples/Quicksort.thy
@@ -1,0 +1,150 @@
+(******************************************************************************
+ * Clean
+ *
+ * Copyright (c) 2018-2019 Université Paris-Saclay, Univ. Paris-Sud, France
+ *
+ * All rights reserved.
+ *
+ * Redistribution and use in source and binary forms, with or without
+ * modification, are permitted provided that the following conditions are
+ * met:
+ *
+ *     * Redistributions of source code must retain the above copyright
+ *       notice, this list of conditions and the following disclaimer.
+ *
+ *     * Redistributions in binary form must reproduce the above
+ *       copyright notice, this list of conditions and the following
+ *       disclaimer in the documentation and/or other materials provided
+ *       with the distribution.
+ *
+ *     * Neither the name of the copyright holders nor the names of its
+ *       contributors may be used to endorse or promote products derived
+ *       from this software without specific prior written permission.
+ *
+ * THIS SOFTWARE IS PROVIDED BY THE COPYRIGHT HOLDERS AND CONTRIBUTORS
+ * "AS IS" AND ANY EXPRESS OR IMPLIED WARRANTIES, INCLUDING, BUT NOT
+ * LIMITED TO, THE IMPLIED WARRANTIES OF MERCHANTABILITY AND FITNESS FOR
+ * A PARTICULAR PURPOSE ARE DISCLAIMED. IN NO EVENT SHALL THE COPYRIGHT
+ * OWNER OR CONTRIBUTORS BE LIABLE FOR ANY DIRECT, INDIRECT, INCIDENTAL,
+ * SPECIAL, EXEMPLARY, OR CONSEQUENTIAL DAMAGES (INCLUDING, BUT NOT
+ * LIMITED TO, PROCUREMENT OF SUBSTITUTE GOODS OR SERVICES; LOSS OF USE,
+ * DATA, OR PROFITS; OR BUSINESS INTERRUPTION) HOWEVER CAUSED AND ON ANY
+ * THEORY OF LIABILITY, WHETHER IN CONTRACT, STRICT LIABILITY, OR TORT
+ * (INCLUDING NEGLIGENCE OR OTHERWISE) ARISING IN ANY WAY OUT OF THE USE
+ * OF THIS SOFTWARE, EVEN IF ADVISED OF THE POSSIBILITY OF SUCH DAMAGE.
+ ******************************************************************************)
+
+(*
+ * Quicksort : all at a glance. 
+ *
+ * Authors : Burkhart Wolff, Frédéric Tuong
+ *)
+
+chapter \<open> Clean Semantics : A Coding-Concept Example\<close>
+
+text\<open>The following show-case introduces subsequently a non-trivial example involving
+local and global variable declarations, declarations of operations with pre-post conditions as
+well as direct-recursive operations (i.e. C-like functions with side-effects on global and
+local variables. \<close>
+
+theory Quicksort
+  imports Clean.Clean
+          Clean.Hoare_Clean
+          Clean.Clean_Symbex
+begin
+
+section\<open>The Quicksort Example - At a Glance\<close>
+
+text\<open> We present the following quicksort algorithm in some conceptual, high-level notation:
+
+\begin{isar}
+algorithm (A,i,j) =
+    tmp := A[i];
+    A[i]:=A[j];
+    A[j]:=tmp
+
+algorithm partition(A, lo, hi) is
+    pivot := A[hi]
+    i := lo
+    for j := lo to hi - 1 do
+        if A[j] < pivot then
+            swap A[i] with A[j]
+            i := i + 1
+    swap A[i] with A[hi]
+    return i
+
+algorithm quicksort(A, lo, hi) is
+    if lo < hi then
+        p := partition(A, lo, hi)
+        quicksort(A, lo, p - 1)
+        quicksort(A, p + 1, hi)
+
+\end{isar}
+\<close>
+
+
+section\<open>Clean Encoding of the Global State of Quicksort\<close>
+
+
+global_vars state
+    A :: "int list"
+
+function_spec swap (i::nat,j::nat) \<comment> \<open>TODO: the hovering on parameters produces a number of report equal to the number of \<^ML>\<open>Proof_Context.add_fixes\<close> called in \<^ML>\<open>Function_Specification_Parser.checkNsem_function_spec\<close>\<close>
+pre          "\<open>i < length A \<and> j < length A\<close>"    
+post         "\<open>\<lambda>res. length A = length(old A) \<and> res = ()\<close>" 
+local_vars   tmp :: int 
+defines      " \<open> tmp := A ! i\<close>  ;-
+               \<open> A := list_update A i (A ! j)\<close> ;- 
+               \<open> A := list_update A j tmp\<close> " 
+
+
+function_spec partition (lo::nat, hi::nat) returns nat
+pre          "\<open>lo < length A \<and> hi < length A\<close>"    
+post         "\<open>\<lambda>res::nat. length A = length(old A) \<and> res = 3\<close>" 
+local_vars   pivot  :: int
+             i      :: nat
+             j      :: nat
+defines      " \<open>pivot := A ! hi \<close>  ;- \<open>i := lo \<close> ;- \<open>j := lo \<close> ;-
+               while\<^sub>C \<open>j \<le> hi - 1 \<close> 
+                do if\<^sub>C \<open>A ! j < pivot\<close>  
+                     then call\<^sub>C swap \<open>(i , j) \<close>  ;-
+                          \<open>i := i + 1 \<close>
+                     else skip\<^sub>S\<^sub>E 
+                   fi ;-
+                    \<open>j := j + 1 \<close> 
+                od;-
+                call\<^sub>C swap \<open>(i, j)\<close>  ;-
+                return\<^bsub>local_partition_state.result_value_update\<^esub> \<open>i\<close>" 
+
+thm partition_core_def
+
+
+rec_function_spec quicksort (lo::nat, hi::nat) returns unit
+pre          "\<open>lo \<le> hi \<and> hi < length A\<close>"
+post         "\<open>\<lambda>res::unit. \<forall>i\<in>{lo .. hi}. \<forall>j\<in>{lo .. hi}. i \<le> j \<longrightarrow> A!i \<le> A!j\<close>"
+variant      "hi - lo" 
+local_vars   p :: "nat" 
+defines      " if\<^sub>C \<open>lo < hi\<close>  
+               then (p\<^sub>t\<^sub>m\<^sub>p \<leftarrow> call\<^sub>C partition \<open>(lo, hi)\<close> ; assign_local p_update (\<lambda>\<sigma>. p\<^sub>t\<^sub>m\<^sub>p)) ;-
+                     call\<^sub>C quicksort \<open>(lo, p - 1)\<close> ;-
+                     call\<^sub>C quicksort \<open>(lo, p + 1)\<close>  
+               else skip\<^sub>S\<^sub>E 
+               fi"
+
+
+thm quicksort_core_def
+thm quicksort_def
+thm quicksort_pre_def
+thm quicksort_post_def
+
+section\<open>Possible Application Sketch\<close>
+
+lemma quicksort_correct : 
+  "\<lbrace>\<lambda>\<sigma>.   \<triangleright> \<sigma> \<and> quicksort_pre (lo, hi)(\<sigma>) \<and> \<sigma> = \<sigma>\<^sub>p\<^sub>r\<^sub>e \<rbrace> 
+     quicksort (lo, hi) 
+   \<lbrace>\<lambda>r \<sigma>. \<triangleright> \<sigma> \<and> quicksort_post(lo, hi)(\<sigma>\<^sub>p\<^sub>r\<^sub>e)(\<sigma>)(r) \<rbrace>"
+   oops
+
+
+
+end
