thys/Clean/src/Clean_Symbex.thy
@@ -48,12 +48,12 @@ text\<open>  As they are equalities, they can also
 be used as program optimization rules. \<close>
 
 lemma non_exec_assign  : 
-assumes "\<not> exec_stop \<sigma>"
+assumes "\<triangleright> \<sigma>"
 shows "(\<sigma> \<Turnstile> ( _ \<leftarrow> assign f; M)) = ((f \<sigma>) \<Turnstile>  M)"
 by (simp add: assign_def assms exec_bind_SE_success)
 
 lemma non_exec_assign'  : 
-assumes "\<not> exec_stop \<sigma>"
+assumes "\<triangleright> \<sigma>"
 shows "(\<sigma> \<Turnstile> (assign f;- M)) = ((f \<sigma>) \<Turnstile>  M)"
 by (simp add: assign_def assms exec_bind_SE_success bind_SE'_def)
 
@@ -70,12 +70,12 @@ by (simp add: assign_def assms exec_bind_SE_success bind_SE'_def)
 subsection\<open>Assign Execution Rules.  \<close>
 
 lemma non_exec_assign_global  : 
-assumes "\<not> exec_stop \<sigma>"
+assumes "\<triangleright> \<sigma>"
 shows   "(\<sigma> \<Turnstile> ( _ \<leftarrow> assign_global upd rhs; M)) = ((upd (\<lambda>_. rhs \<sigma>) \<sigma>) \<Turnstile>  M)"
 by(simp add: assign_global_def non_exec_assign assms)
 
 lemma non_exec_assign_global'  : 
-assumes "\<not> exec_stop \<sigma>"
+assumes "\<triangleright> \<sigma>"
 shows   "(\<sigma> \<Turnstile> (assign_global upd rhs;- M)) = ((upd (\<lambda>_. rhs \<sigma>) \<sigma>) \<Turnstile>  M)"
   by (metis (full_types) assms bind_SE'_def non_exec_assign_global)
 
@@ -91,13 +91,13 @@ shows   "(\<sigma> \<Turnstile> (assign_global upd rhs;- M)) = ( \<sigma> \<Turn
   by (simp add: assign_global_def assign_def assms exec_bind_SE_success bind_SE'_def)
 
 lemma non_exec_assign_local  : 
-assumes "\<not> exec_stop \<sigma>"
-shows   "(\<sigma> \<Turnstile> ( _ \<leftarrow> assign_local upd rhs; M)) = ((upd (map_hd (\<lambda>_. rhs \<sigma>)) \<sigma>) \<Turnstile>  M)"
+assumes "\<triangleright> \<sigma>"
+shows   "(\<sigma> \<Turnstile> ( _ \<leftarrow> assign_local upd rhs; M)) = ((upd (upd_hd (\<lambda>_. rhs \<sigma>)) \<sigma>) \<Turnstile>  M)"
   by(simp add: assign_local_def non_exec_assign assms)
 
 lemma non_exec_assign_local'  : 
-assumes "\<not> exec_stop \<sigma>"
-shows   "(\<sigma> \<Turnstile> (assign_local upd rhs;- M)) = ((upd (map_hd (\<lambda>_. rhs \<sigma>)) \<sigma>) \<Turnstile>  M)"
+assumes "\<triangleright> \<sigma>"
+shows   "(\<sigma> \<Turnstile> (assign_local upd rhs;- M)) = ((upd (upd_hd (\<lambda>_. rhs \<sigma>)) \<sigma>) \<Turnstile>  M)"
   by (metis assms bind_SE'_def non_exec_assign_local)
 
 lemmas non_exec_assign_localD'= non_exec_assign[THEN iffD1]
@@ -179,67 +179,67 @@ shows   "(\<sigma> \<Turnstile> (call_2\<^sub>C M A\<^sub>1 A\<^sub>2;- M')) = (
 subsection\<open>Basic Call Symbolic Execution Rules.  \<close>
 
 lemma non_exec_call_0  : 
-assumes "\<not> exec_stop \<sigma>"
+assumes "\<triangleright> \<sigma>"
 shows   "(\<sigma> \<Turnstile> ( _ \<leftarrow> call_0\<^sub>C M; M')) = (\<sigma> \<Turnstile> M;- M')"
   by (simp add: assms bind_SE'_def bind_SE_def call_0\<^sub>C_def valid_SE_def)
 
 lemma non_exec_call_0'  : 
-assumes "\<not> exec_stop \<sigma>"
+assumes "\<triangleright> \<sigma>"
 shows   "(\<sigma> \<Turnstile> call_0\<^sub>C M;- M') = (\<sigma> \<Turnstile> M;- M')"
   by (simp add: assms bind_SE'_def non_exec_call_0)
 
 lemma non_exec_call_1  : 
-assumes "\<not> exec_stop \<sigma>"
-shows   "(\<sigma> \<Turnstile> ( x \<leftarrow> (call_1\<^sub>C M A\<^sub>1); M' x)) = (\<sigma> \<Turnstile> (x \<leftarrow> M (A\<^sub>1 \<sigma>); M' x))"
+assumes "\<triangleright> \<sigma>"
+shows   "(\<sigma> \<Turnstile> ( x \<leftarrow> (call_1\<^sub>C M (A\<^sub>1)); M' x)) = (\<sigma> \<Turnstile> (x \<leftarrow> M (A\<^sub>1 \<sigma>); M' x))"
   by (simp add: assms bind_SE'_def call\<^sub>C_def bind_SE_def call_1\<^sub>C_def valid_SE_def)
 
 lemma non_exec_call_1'  : 
-assumes "\<not> exec_stop \<sigma>"
-shows   "(\<sigma> \<Turnstile> call_1\<^sub>C M A\<^sub>1;- M') = (\<sigma> \<Turnstile>  M (A\<^sub>1 \<sigma>);- M')"
+assumes "\<triangleright> \<sigma>"
+shows   "(\<sigma> \<Turnstile> call_1\<^sub>C M (A\<^sub>1);- M') = (\<sigma> \<Turnstile>  M (A\<^sub>1 \<sigma>);- M')"
   by (simp add: assms bind_SE'_def non_exec_call_1)
 
-
+(* general case *)
 lemma non_exec_call  : 
-assumes "\<not> exec_stop \<sigma>"
-shows   "(\<sigma> \<Turnstile> ( x \<leftarrow> (call\<^sub>C M A\<^sub>1); M' x)) = (\<sigma> \<Turnstile> (x \<leftarrow> M (A\<^sub>1 \<sigma>); M' x))"
+assumes "\<triangleright> \<sigma>"
+shows   "(\<sigma> \<Turnstile> ( x \<leftarrow> (call\<^sub>C M (A\<^sub>1)); M' x)) = (\<sigma> \<Turnstile> (x \<leftarrow> M (A\<^sub>1 \<sigma>); M' x))"
   by (simp add: assms call\<^sub>C_def bind_SE'_def bind_SE_def call_1\<^sub>C_def valid_SE_def)
 
 lemma non_exec_call'  : 
-assumes "\<not> exec_stop \<sigma>"
-shows   "(\<sigma> \<Turnstile> call\<^sub>C M A\<^sub>1;- M') = (\<sigma> \<Turnstile>  M (A\<^sub>1 \<sigma>);- M')"
+assumes "\<triangleright> \<sigma>"
+shows   "(\<sigma> \<Turnstile> call\<^sub>C M (A\<^sub>1);- M') = (\<sigma> \<Turnstile>  M (A\<^sub>1 \<sigma>);- M')"
   by (simp add: assms bind_SE'_def non_exec_call)
 
 
 lemma non_exec_call_2  : 
-assumes "\<not> exec_stop \<sigma>"
-shows   "(\<sigma> \<Turnstile> ( _ \<leftarrow> (call_2\<^sub>C M A\<^sub>1 A\<^sub>2); M')) = (\<sigma> \<Turnstile> M (A\<^sub>1 \<sigma>) (A\<^sub>2 \<sigma>);- M')"
+assumes "\<triangleright> \<sigma>"
+shows   "(\<sigma> \<Turnstile> ( _ \<leftarrow> (call_2\<^sub>C M (A\<^sub>1) (A\<^sub>2)); M')) = (\<sigma> \<Turnstile> M (A\<^sub>1 \<sigma>) (A\<^sub>2 \<sigma>);- M')"
   by (simp add: assms bind_SE'_def bind_SE_def call_2\<^sub>C_def valid_SE_def)
 
 lemma non_exec_call_2'  : 
-assumes "\<not> exec_stop \<sigma>"
-shows   "(\<sigma> \<Turnstile> call_2\<^sub>C M A\<^sub>1 A\<^sub>2;- M') = (\<sigma> \<Turnstile>  M (A\<^sub>1 \<sigma>) (A\<^sub>2 \<sigma>);- M')"
+assumes "\<triangleright> \<sigma>"
+shows   "(\<sigma> \<Turnstile> call_2\<^sub>C M (A\<^sub>1) (A\<^sub>2);- M') = (\<sigma> \<Turnstile>  M (A\<^sub>1 \<sigma>) (A\<^sub>2 \<sigma>);- M')"
   by (simp add: assms bind_SE'_def non_exec_call_2)
 
 
 subsection\<open>Conditional.  \<close>
 
 lemma exec_If\<^sub>C_If\<^sub>S\<^sub>E  : 
-assumes "\<not> exec_stop \<sigma>"
-shows  " ((if\<^sub>C P then B\<^sub>1 else B\<^sub>2 fi))\<sigma> = ((if\<^sub>S\<^sub>E P then B\<^sub>1 else B\<^sub>2 fi)) \<sigma> "
+assumes "\<triangleright> \<sigma>"
+shows   "((if\<^sub>C P then B\<^sub>1 else B\<^sub>2 fi))\<sigma> = ((if\<^sub>S\<^sub>E P then B\<^sub>1 else B\<^sub>2 fi)) \<sigma> "
   unfolding if_SE_def MonadSE.if_SE_def Symbex_MonadSE.valid_SE_def MonadSE.bind_SE'_def
   by (simp add: assms bind_SE_def if_C_def)
     
     
 lemma valid_exec_If\<^sub>C  : 
-assumes "\<not> exec_stop \<sigma>"
-shows  "(\<sigma> \<Turnstile> (if\<^sub>C P then B\<^sub>1 else B\<^sub>2 fi);-M) = (\<sigma> \<Turnstile> (if\<^sub>S\<^sub>E P then B\<^sub>1 else B\<^sub>2 fi);-M)"
+assumes "\<triangleright> \<sigma>"
+shows   "(\<sigma> \<Turnstile> (if\<^sub>C P then B\<^sub>1 else B\<^sub>2 fi);-M) = (\<sigma> \<Turnstile> (if\<^sub>S\<^sub>E P then B\<^sub>1 else B\<^sub>2 fi);-M)"
   by (meson assms exec_If\<^sub>C_If\<^sub>S\<^sub>E valid_bind'_cong)
 
 
       
 lemma exec_If\<^sub>C'  : 
 assumes "exec_stop \<sigma>"
-shows  "(\<sigma> \<Turnstile> (if\<^sub>C P then B\<^sub>1 else B\<^sub>2 fi);-M) = (\<sigma> \<Turnstile> M)"    
+shows   "(\<sigma> \<Turnstile> (if\<^sub>C P then B\<^sub>1 else B\<^sub>2 fi);-M) = (\<sigma> \<Turnstile> M)"    
   unfolding if_SE_def MonadSE.if_SE_def Symbex_MonadSE.valid_SE_def MonadSE.bind_SE'_def bind_SE_def
     by (simp add: assms if_C_def)
     
@@ -252,52 +252,51 @@ shows  "(\<sigma> \<Turnstile> (while\<^sub>C P do B\<^sub>1 od);-M) = (\<sigma>
 
     
     
-lemma if\<^sub>C_cond_cong : "f \<sigma> = g \<sigma> \<Longrightarrow> 
-                           (if\<^sub>C f then c else d fi) \<sigma> = 
-                           (if\<^sub>C g then c else d fi) \<sigma>"
+lemma if\<^sub>C_cond_cong : "f \<sigma> = g \<sigma> \<Longrightarrow> (if\<^sub>C f then c else d fi) \<sigma> = 
+                                     (if\<^sub>C g then c else d fi) \<sigma>"
   unfolding if_C_def
    by simp 
    
  
 subsection\<open>Break - Rules.  \<close>
 
-lemma break_assign_skip [simp]: "break ;- assign f = break"
+lemma break_assign_skip [simp]: "(break ;- assign f) = break"
   apply(rule ext)
   unfolding break_def assign_def exec_stop_def bind_SE'_def   bind_SE_def
   by auto
 
 
 
-lemma break_if_skip [simp]: "break ;- (if\<^sub>C b then c else d fi) = break"
+lemma break_if_skip [simp]: "(break ;- if\<^sub>C b then c else d fi) = break"
   apply(rule ext)
   unfolding break_def assign_def exec_stop_def if_C_def bind_SE'_def   bind_SE_def
   by auto
     
                        
-lemma break_while_skip [simp]: "break ;- (while\<^sub>C b do c od) = break"
+lemma break_while_skip [simp]: "(break ;- while\<^sub>C b do c od) = break"
   apply(rule ext)
   unfolding while_C_def skip\<^sub>S\<^sub>E_def unit_SE_def bind_SE'_def bind_SE_def break_def exec_stop_def
   by simp
 
     
 lemma unset_break_idem [simp] : 
- "( unset_break_status ;- unset_break_status ;- M) = (unset_break_status ;- M)"
+ "(unset_break_status ;- unset_break_status ;- M) = (unset_break_status ;- M)"
   apply(rule ext)  unfolding unset_break_status_def bind_SE'_def bind_SE_def by auto
 
 lemma return_cancel1_idem [simp] : 
- "( return\<^sub>C X E ;- assign_global X E' ;- M) = ( return\<^sub>C X E ;- M)"
+ "(return\<^bsub>X\<^esub>(E) ;- X :==\<^sub>G E' ;- M) = ( return\<^sub>C X E ;- M)"
   apply(rule ext, rename_tac "\<sigma>")  
   unfolding unset_break_status_def bind_SE'_def bind_SE_def
-            assign_def return\<^sub>C_def assign_global_def assign_local_def
+            assign_def return\<^sub>C_def return\<^sub>C0_def assign_global_def assign_local_def
   apply(case_tac "exec_stop \<sigma>")
   apply auto
   by (simp add: exec_stop_def set_return_status_def)
     
 lemma return_cancel2_idem [simp] : 
- "( return\<^sub>C X E ;- assign_local X E' ;- M) = ( return\<^sub>C X E ;- M)"
+ "( return\<^bsub>X\<^esub>(E) ;- X :==\<^sub>L E' ;- M) = ( return\<^sub>C X E ;- M)"
     apply(rule ext, rename_tac "\<sigma>")  
   unfolding unset_break_status_def bind_SE'_def bind_SE_def
-            assign_def return\<^sub>C_def assign_global_def assign_local_def
+            assign_def return\<^sub>C_def return\<^sub>C0_def assign_global_def assign_local_def
   apply(case_tac "exec_stop \<sigma>")
    apply auto
   by (simp add: exec_stop_def set_return_status_def)
