thys/Clean/src/Optics.thy
@@ -1,0 +1,47 @@
+text\<open>This is an excerpt of the Optics library 
+     \<^url>\<open>https://www.isa-afp.org/entries/Optics.html\<close> by Frank Zeyda and
+     Simon Foster. It provides a rich infrastructure for \<^emph>\<open>algebraic lenses\<close>,
+     an abstract theory allowing to describe parts of memory and their 
+     independence. We use it to abstractly model typed program variables and
+     framing conditions. 
+
+     Optics provides a rich framework for lense compositions and sub-lenses
+     which we will not use in the context of Clean; even the offered concept
+     of a list-lense, a possible means to model the stack-infrastructure 
+     required for local variables, is actually richer than needed.
+
+     Since Clean strives for minimality, we restrict ourselves to this "proxy"
+     theory for Optics.
+\<close>
+
+theory Optics
+  imports Lens_Laws
+begin
+
+
+fun      upd_hd :: "('a \<Rightarrow> 'a) \<Rightarrow> 'a list \<Rightarrow> 'a list" 
+  where "upd_hd f [] = []"
+      | "upd_hd f (a#S) = f a # S"
+
+lemma [simp] :"tl (upd_hd f S) = tl S" 
+  by (metis list.sel(3) upd_hd.elims)
+
+
+definition upd2put :: "(('d \<Rightarrow> 'b) \<Rightarrow> 'a \<Rightarrow> 'c) \<Rightarrow> 'a \<Rightarrow> 'b \<Rightarrow> 'c"
+  where   "upd2put f = (\<lambda>\<sigma>. \<lambda> b. f (\<lambda>_. b) \<sigma>)"
+
+definition create\<^sub>L 
+  where "create\<^sub>L getv updv = \<lparr>lens_get = getv,lens_put = upd2put updv\<rparr>"
+
+definition "hd\<^sub>L = create\<^sub>L hd upd_hd"   (* works since no partial lenses needed in Clean*)
+
+definition "map_nth i = (\<lambda>f l. list_update l i (f (l ! i)))"
+
+lemma indep_list_lift : 
+     "X \<bowtie> create\<^sub>L getv updv 
+      \<Longrightarrow> (\<lambda>f \<sigma>. updv (\<lambda>_. f (getv \<sigma>)) \<sigma>) = updv 
+      \<Longrightarrow> X \<bowtie> create\<^sub>L (hd \<circ> getv ) (updv \<circ> upd_hd)"
+  unfolding create\<^sub>L_def o_def Lens_Laws.lens_indep_def upd2put_def
+  by (auto,metis (no_types)) (metis (no_types))
+
+end
